theories/coneris/examples/bloom_filter/concurrent_bloom_filter_alt.v
@@ -1,0 +1,417 @@
+From iris.base_logic.lib Require Import invariants.
+From iris.algebra Require Import gset_bij auth excl frac agree numbers.
+From clutch.coneris Require Import coneris par spawn spin_lock hash atomic lock concurrent_hash con_hash_interface4 bloom_filter.
+From clutch.coneris.lib Require Import list array.
+
+Set Default Proof Using "Type*".
+
+
+
+Section conc_bloom_filter.
+
+
+
+  Variables filter_size max_key num_hash num_threads : nat.
+  Context `{!conerisGS Σ, !spawnG Σ, c:con_hash4 Σ filter_size, !inG Σ (excl_authR boolO), !inG Σ (prodR fracR val0) }.
+
+
+  Definition init_bloom_filter : expr :=
+    λ: "_" ,
+      let: "hfuns" := list_seq_fun #0 #num_hash (λ: "_", init_hash4 #()) in
+      let: "arr" := array_init #(S filter_size) (λ: "x", #false)%E in
+      let: "l" := ref ("hfuns", "arr") in
+      "l".
+
+  Definition insert_bloom_filter : expr :=
+    λ: "l" "v" ,
+      let, ("hfuns", "arr") := !"l" in
+      list_iter (λ: "h",
+          let: "i" := "h" "v" in
+          "arr" +ₗ "i" <- #true) "hfuns".
+
+
+  Definition lookup_bloom_filter : expr :=
+    λ: "l" "v" ,
+      let, ("hfuns", "arr") := !"l" in
+      let: "res" := ref #true in
+      list_iter (λ: "h",
+          let: "i" := "h" "v" in
+          if: !("arr" +ₗ "i") then #() else "res" <- #false) "hfuns" ;;
+      !"res".
+
+(*
+  (*
+     The invariant of the case study keeps track of three sets, s1, s2, and s3, whose union s is always constant.
+       - s1 represents the set of elements that are in the tape of some hash
+       - s2 represents the set of indices that have been read from the hash, but are still waiting to be written to
+       the array
+       - s3 represents the set of indices of the array that have been set to 1
+
+     After the initialization, s1 will contain all elements in the hash sets, while s2 and s3 are empty. The deterministic
+     part of the program will just advance the physical state of the bloom filter so that at the end s1 and s2 are empty.
+
+     Additionally, the invariant ensures that every thread reading from a hash will find a non-empty tape (and therefore there
+     is no more sampling happening).
+   *)
+  Definition bloom_filter_inv (s : gset nat) (a : loc) (arr lbls : list val) (snames : list hash_set_gname) (tnames : list hash_tape_gname): iProp Σ :=
+    ∃ (s1 s2 s3 : gset nat),
+      ⌜ s1 ∪ s2 ∪ s3 = s ⌝ ∗
+      (* Every element in s1 is in the tape of some hash *)
+      ([∗ list] x ∈ (zip lbls (zip snames tnames)),
+           ∃ (sx : list nat), hash_tape1 (fst x) sx (fst (snd x)) (snd (snd x)) ∗ ⌜ subseteq (list_to_set sx) s1 ⌝) ∗
+      (* Every element in s2 is waiting to be written *)
+      (* Every element in s3 is an index set to 1 in the array *)
+      (a ↦∗ arr) ∗
+      ⌜ forall i, arr !! i = Some #true -> i ∈ s3  ⌝ ∗
+      ⌜ forall i, i ∈ s3 -> (i < S filter_size)%nat  ⌝ ∗
+      ([∗ set] x ∈ s3, ∃ γ, (hash_set_frag1 x γ)).
+ *)
+
+
+  Lemma hash_frag_valid k v γ :
+    hash_frag4 k v γ  -∗ ⌜ (v ≤ filter_size)%nat ⌝.
+  Admitted.
+
+  Definition con_hash_inv_list N hfs hnames ks (s : gset nat) :=
+    ([∗ list] i ↦f;γ ∈ hfs;hnames,
+       ∃ lk hm,
+         con_hash_inv4 N f lk hm (λ _, True) γ.1 γ.2 ∗
+         ([∗ list] k ∈ ks, ∃ v, ⌜ v ∈ s ⌝ ∗ hash_frag4 k v γ.1))%I.
+
+
+  Lemma con_hash_inv_list_cons N f fs2 hnames ks s :
+    con_hash_inv_list N ((f :: fs2)) hnames ks s -∗
+    (∃ lk hm γ hnames2,
+        ⌜ hnames = γ :: hnames2 ⌝ ∗
+        con_hash_inv4 N f lk hm (λ _, True) γ.1 γ.2 ∗
+        ([∗ list] k ∈ ks, ∃ v, ⌜ v ∈ s ⌝ ∗ hash_frag4 k v γ.1) ∗
+        con_hash_inv_list N fs2 hnames2 ks s
+    ).
+  Admitted.
+
+  Definition bloom_filter_inv_aux N bfl hfuns a
+    (hnames : list (hash_view_gname * hash_lock_gname)) ks (s : gset nat) : iPropI Σ :=
+        (∃ hfs,
+            (bfl ↦ (hfuns, LitV (LitLoc a))%V ∗
+            ⌜ is_list_HO hfs hfuns ⌝ ∗
+            ⌜ length hfs = num_hash ⌝ ∗
+            con_hash_inv_list N hfs hnames ks s ∗
+            ⌜ forall i, i ∈ s -> (i < S filter_size)%nat  ⌝ ∗
+            (∃ (arr : list val),
+                 (a ↦∗ arr) ∗
+                 ⌜ length arr = S filter_size ⌝ ∗
+                 ⌜ forall i, i < S filter_size -> arr !! i = Some #true -> i ∈ s  ⌝)))%I.
+
+  Definition bloom_filter_inv N bfl hfuns a
+    (hnames : list (hash_view_gname * hash_lock_gname)) ks (s : gset nat) : iPropI Σ :=
+      (inv (N.@"bf") (bloom_filter_inv_aux N bfl hfuns a hnames ks s)).
+
+
+(*
+  Definition con_hash_inv_list N hfs hnames :=
+      ([∗ list] k↦hf;γ ∈ hfs;hnames,
+        ∃ f α lk hm ns,
+          ⌜ hf = (f, α)%V ⌝ ∗
+          hash_tape1 α ns γ.2.1 γ.2.2.1 ∗
+        con_hash_inv1 N f lk hm (λ _, True) γ.1 γ.2.1 γ.2.2.1 γ.2.2.2)%I.
+
+
+
+*)
+
+
+  Lemma hash_preview_list N rem (ks : list nat) f l hm R {HR: ∀ m, Timeless (R m )} m γ_hv γ_lock (bad : gset nat) E:
+     ↑(N) ⊆ E ->
+     (forall x : nat, x ∈ bad -> (x < S filter_size)%nat) ->
+     hash_auth4 m γ_hv -∗
+     con_hash_inv4 N f l hm R γ_hv γ_lock -∗
+     ⌜ NoDup ks ⌝ -∗
+     ([∗ list] k ∈ ks,  ⌜ m !! k = None ⌝) -∗
+     ↯ (fp_error filter_size num_hash (rem + length ks) (size bad)) -∗
+     state_update E E (∃ (res : gset nat),
+          ⌜ forall x : nat, x ∈ (bad ∪ res) -> (x < S filter_size)%nat ⌝ ∗
+          ↯ (fp_error filter_size num_hash rem (size (bad ∪ res))) ∗
+          ([∗ list] k ∈ ks, ∃ v, ⌜ v ∈ (bad ∪ res) ⌝ ∗ hash_frag4 k v γ_hv )).
+  Proof.
+    iIntros (Hsubset Hbound) "Hhauth #Hhinv".
+    iInduction ks as [|k ks] "IH" forall (m bad Hbound).
+    - iIntros "Hndup Hnone Herr".
+      rewrite /= Nat.add_0_r.
+      iModIntro.
+      iExists bad.
+      replace (bad ∪ bad) with bad by set_solver.
+      iSplit; auto.
+    - iIntros "%Hndup (Hknone & Hksnone) Herr".
+      pose proof (NoDup_cons_1_1 k ks Hndup) as Hdup1.
+      pose proof (NoDup_cons_1_2 k ks Hndup) as Hdup2.
+      replace (rem + length (k :: ks)) with (S rem + (length ks));
+        [|simpl; lia].
+      assert (forall m b, 0 <= fp_error filter_size num_hash m b)%R as Hfp.
+      {
+        intros; apply fp_error_bounded.
+      }
+      iPoseProof (hash_preview4 N k _ _ _ _ _ _ _ bad
+                      (mknonnegreal (fp_error filter_size num_hash (S rem + length ks) (size bad))
+                         (Hfp _ _))
+                      (mknonnegreal (fp_error filter_size num_hash (rem + length ks) (size bad))
+                         (Hfp _ _))
+                      (mknonnegreal (fp_error filter_size num_hash (rem + length ks) (S (size bad)))
+                         (Hfp _ _))
+                      E with "Hhauth Hhinv Hknone [Herr]") as "Hcur"; auto; try done.
+       + simpl.
+         case_bool_decide.
+         * rewrite fp_error_max /=; auto.
+           rewrite fp_error_max /=; auto.
+           rewrite !Rmult_1_l.
+           lra.
+         * right.
+           rewrite (Rmult_comm (size bad / (filter_size + 1))).
+           rewrite (Rmult_comm ((filter_size + 1 - size bad) / (filter_size + 1))).
+           rewrite Rmult_plus_distr_r.
+           rewrite !(Rmult_assoc _ _ (filter_size + 1)).
+           rewrite !Rinv_l; [lra|].
+           real_solver.
+       + iMod ("Hcur") as "(%v & [(%Hnotbad & Herr)|(%Hbad & Herr)] & Hhauth)".
+         ** simpl.
+            iPoseProof (hash_auth_duplicate _ k v with "Hhauth") as "#Hkv";
+              [rewrite lookup_insert // |].
+            iMod ("IH" $! _ bad with "[] Hhauth [] [Hksnone] Herr") as "(%res&?&?&?)"; auto.
+            {
+              iApply (big_sepL_mono with "Hksnone").
+              iIntros (i k' Hsome) "%Hk'".
+              iPureIntro.
+              rewrite lookup_insert_ne; auto.
+              apply elem_of_list_lookup_2 in Hsome.
+              apply NoDup_cons_1_1 in Hndup.
+              set_solver.
+            }
+            iModIntro.
+            iExists (bad ∪ res).
+            replace (bad ∪ (bad ∪ res)) with (bad ∪ res) by set_solver.
+            iFrame.
+            iExists v.
+            iSplit; auto.
+            iPureIntro.
+            set_solver.
+         ** simpl.
+            iPoseProof (hash_auth_duplicate _ k v with "Hhauth") as "#Hkv";
+              [rewrite lookup_insert // |].
+            iMod ("IH" $! _ (bad ∪ {[fin_to_nat v]}) with "[] Hhauth [] [Hksnone] [Herr]") as "(%res&?&?&?)"; auto.
+            *** iPureIntro.
+                intros x Hx.
+                apply elem_of_union in Hx as [Hx|Hx]; auto.
+                apply elem_of_singleton in Hx as ->.
+                apply fin_to_nat_lt.
+            *** iApply (big_sepL_mono with "Hksnone").
+                iIntros (i k' Hsome) "%Hk'".
+                iPureIntro.
+                rewrite lookup_insert_ne; auto.
+                apply elem_of_list_lookup_2 in Hsome.
+                apply NoDup_cons_1_1 in Hndup.
+                set_solver.
+            *** rewrite size_union; [|set_solver].
+                rewrite size_singleton.
+                replace (size bad + 1) with (S (size bad)) by lia.
+                iFrame.
+            *** iModIntro.
+                iExists ((bad ∪ {[fin_to_nat v]}) ∪ res).
+                replace (bad ∪ (bad ∪ {[fin_to_nat v]} ∪ res)) with ((bad ∪ {[fin_to_nat v]}) ∪ res) by set_solver.
+                iFrame.
+                iExists (fin_to_nat v).
+                iSplit; auto.
+                iPureIntro.
+                set_solver.
+  Qed.
+
+
+  Lemma bloom_filter_init_spec N (ks : list nat) :
+    (length ks = num_threads) ->
+    NoDup ks ->
+    ([∗ list] k ∈ ks, ⌜ (k ≤ max_key)%nat ⌝) -∗
+    {{{ ↯ (fp_error filter_size num_hash (num_hash * num_threads) 0) }}}
+      init_bloom_filter #()
+   {{{ (bfl:loc), RET #bfl ;
+         ∃ hfuns a hnames s,
+           bloom_filter_inv N bfl hfuns a hnames ks s
+   }}}.
+   Proof.
+    iIntros (Hthreads Hndup) "#Hks".
+    iIntros (Φ).
+    iModIntro.
+    iIntros "Herr HΦ".
+    rewrite /init_bloom_filter.
+    wp_pures.
+    set (Ψ := (λ l, ⌜ num_hash < length l ⌝ ∨
+                (∃ (s : gset nat),
+                      ↯(fp_error filter_size num_hash ((num_hash - length l) * num_threads) (size s)) ∗
+                      ⌜ ∀ x : nat, x ∈ s → x < S filter_size ⌝ ∗
+                      ([∗ list] f ∈ l,
+                        (∃ lk hm γ, con_hash_inv4 N f lk hm (λ _, True) γ.1 γ.2 ∗
+                            ([∗ list] k ∈ ks, ∃ v, ⌜ v ∈ s ⌝ ∗ hash_frag4 k v γ.1)))))%I).
+    wp_apply (wp_list_seq_fun_HO_invariant _ Ψ
+                0 num_hash _ (λ _ _, True)%I with "[] [Herr] [HΦ]").
+    - iIntros (i l Ξ).
+      iModIntro.
+      iIntros "HΨ HΞ".
+      wp_pures.
+      iApply pgl_wp_state_update.
+      wp_apply (con_hash_init4 N (λ _, True)%I); auto.
+      iIntros (f) "(%lk & %hm & %γ1 & %γ2 & #Hinv & Hhauth)".
+      iApply "HΞ".
+      iApply (state_update_mono _ _ (Ψ (f :: l))); auto.
+      rewrite /Ψ cons_length.
+      assert (num_hash ≤ length l \/ num_hash > length l) as [Haux|?] by lia.
+      {
+        iModIntro.
+        iDestruct "HΨ" as "[%|HΨ]"; [iLeft; iPureIntro; lia |].
+        iLeft. iPureIntro. lia.
+      }
+      iDestruct "HΨ" as "[%|HΨ]"; [iModIntro; iLeft; iPureIntro; lia |].
+      iDestruct "HΨ" as "(%s & Herr & %Hbound & Hl)".
+      rewrite -Hthreads.
+      replace ((num_hash - length l) * length ks) with ((num_hash - S (length l)) * length ks + length ks);
+        last first.
+      {
+        rewrite -{2}(Nat.mul_1_l (length ks)).
+        rewrite -Nat.mul_add_distr_r.
+        f_equal.
+        lia.
+      }
+      iMod (hash_preview_list N _ ks _ _ _ _ _ _ _ s ⊤ with "Hhauth Hinv [][][Herr]") as "Hupd"; auto.
+      iModIntro.
+      iRight.
+      iDestruct "Hupd" as "(%res & ? & Herr & ?)".
+      iExists (s ∪ res).
+      iFrame.
+      iApply big_sepL_cons.
+      iSplitR "Hl".
+      * iExists lk, hm, (γ1, γ2).
+        auto.
+      * iApply (big_sepL_mono with "Hl").
+        iIntros (k v Hkv) "(%lk' & %hm' & %γ' & Hinv & Hlist)".
+        iExists lk', hm', γ'.
+        iFrame.
+        iApply (big_sepL_mono with "Hlist").
+        iIntros (???) "(%&%&?)".
+        iExists _; iFrame.
+        iPureIntro. set_solver.
+   - rewrite /Ψ.
+     iRight.
+     iExists ∅.
+     rewrite size_empty nil_length Nat.sub_0_r.
+     iFrame.
+     iSplit; [iPureIntro; set_solver |].
+     done.
+   - iModIntro.
+     iIntros (hfuns fαs) "(%Hhfuns & %Hlen & HΨ & _)".
+      wp_pures.
+      wp_apply (wp_array_init (λ _ v, ⌜ v = #false ⌝%I)).
+      + real_solver.
+      + iApply big_sepL_intro.
+        iModIntro.
+        iIntros (??) "?".
+        wp_pures.
+        done.
+      + iIntros (a arr) "(%HlenA & Ha & %Harr)".
+        wp_pures.
+        wp_alloc l as "Hl".
+        wp_pures.
+        rewrite /Ψ.
+        iDestruct "HΨ" as "[%|(%s & Herr & %Hbound & Hfs)]";
+          [lia |].
+        iAssert ([∗ list] f ∈ fαs, ∃ (γ : hash_view_gname * hash_lock_gname) (lk hm : val),
+                    con_hash_inv4 N f lk hm (λ _ : gmap nat nat, True) γ.1 γ.2 ∗
+                      ([∗ list] k ∈ ks, ∃ v : nat, ⌜v ∈ s⌝ ∗ hash_frag4 k v γ.1))%I with "[Hfs]" as "Hfs".
+        {
+          iApply (big_sepL_mono with "Hfs").
+          iIntros (???) "(%&%&%&?)".
+          iFrame.
+        }
+        iPoseProof (array.big_sepL_exists with "Hfs") as "(%hnames & Hfs)"; eauto.
+        iApply "HΦ".
+        iExists hfuns, a.
+        iExists hnames, s.
+        iMod (inv_alloc _ _ (bloom_filter_inv_aux N l hfuns a hnames ks s) with "[Herr Ha Hl Hfs]") as "#Hinv";
+          [| iApply "Hinv"].
+        rewrite /bloom_filter_inv_aux.
+        iModIntro.
+        iExists fαs.
+        iFrame.
+        iPureIntro.
+        repeat split; auto.
+        ** lia.
+        ** intros i Hi1 Hi2.
+           specialize (Harr i #true Hi2).
+           simplify_eq.
+  Qed.
+
+
+  Lemma bloom_filter_insert_thread_spec N bfl hfuns a hnames (k : nat) (ks : list nat) s :
+    (k ∈ ks) ->
+    ([∗ list] k ∈ ks, ⌜ (k ≤ max_key)%nat ⌝) -∗
+      {{{ bloom_filter_inv N bfl hfuns a hnames ks s }}}
+            insert_bloom_filter #bfl #k
+      {{{ RET #(); True  }}}.
+  Proof using c conerisGS0 conerisGS1 excl_authR filter_size inG0 inG1 max_key max_key0 num_hash num_threads spawnG0 val0 Σ.
+    iIntros (Hk Hleq Φ) "!# #Hinv HΦ".
+    rewrite /insert_bloom_filter.
+    wp_pures.
+    wp_bind (! _)%E.
+    iInv "Hinv" as "(%hfs&>Hbfl&>%Hhfs&>%Hlen&#Hhinv&>%Hbound&?)" "Hclose".
+    wp_load.
+    iMod ("Hclose" with "[-HΦ]").
+    {
+      iModIntro.
+      iExists hfs.
+      iFrame.
+      repeat iSplit; auto.
+    }
+    iModIntro.
+    wp_pures.
+    wp_apply (wp_list_iter_invariant_HO
+                (λ fs1 fs2,
+                   ∃ hnames2,
+                    con_hash_inv_list N fs2 hnames2 ks s)%I with "[][][HΦ]"); auto.
+    - iIntros (fs1 f fs2 Ψ) "!# (%hnames2 & Hiter) HΨ".
+      wp_pures.
+      rewrite /con_hash_inv_list.
+      iPoseProof (con_hash_inv_list_cons with "Hiter")
+        as "(%lk&%hm&%γ&%hnames3&->&#Hinvf&Hfrags&Htail)".
+      wp_bind (f _).
+      iPoseProof (big_sepL_elem_of _ _ k with "Hfrags") as "(%v&%Hv&Hfrag)"; auto.
+      wp_apply (con_hash_spec4 with "[$Hfrag //]").
+      iIntros (?) "->".
+      wp_pures.
+      iInv "Hinv" as "(%&?&?&?&?&?&%arr&Harr&>%HlenA&>%Htrue)" "Hclose".
+      wp_apply (wp_store_offset with "[$Harr]").
+      {
+        apply lookup_lt_is_Some_2.
+        rewrite HlenA //.
+        by apply Hbound.
+      }
+      iIntros "Harr".
+      iMod ("Hclose" with "[-HΨ Htail]").
+      {
+        iModIntro.
+        iFrame.
+        iPureIntro.
+        split.
+        - rewrite insert_length //.
+        - intros i Hi Hlookup.
+          destruct (decide (i = v)) as [-> | Hneq]; auto.
+          apply Htrue; auto.
+          by rewrite list_lookup_insert_ne in Hlookup.
+      }
+      iApply "HΨ".
+      iModIntro.
+      rewrite /con_hash_inv_list.
+      iExists hnames3.
+      iFrame.
+
+   - iModIntro.
+     iIntros "?".
+     by iApply "HΦ".
+ Qed.
+
+
+
